theories/Observations.v
@@ -1,0 +1,55 @@
+From Stdlib Require Import
+  Arith   
+  Logic.FunctionalExtensionality         
+  Classes.RelationClasses
+  Morphisms
+  Program.Basics
+  List
+  Lia.
+
+From LEpic Require Import Syntax.
+From LEpic Require Import Contexts.
+
+Inductive obs :=
+| var (r: rvar)
+| emp
+| tup (o1 o2: obs)
+| dcl (mc: maybe_closed) (e: effect)
+| lam (mc: maybe_closed) (es: list effect) (o: obs)
+with
+effect := 
+| eff (f: fvar) (os: list obs)
+with
+maybe_closed := 
+| closed
+| open (rs: list rvar)
+.
+
+Definition machine := prod obs term.
+
+Inductive wf_machine : machine -> Prop :=
+| wf_mach :
+  forall m n
+    (G : lctxt m)
+    (D : lctxt n)
+    (o : obs)
+    (t : term),
+    wf_observation o ->
+    wf_term m n G D t ->
+    wf_machine (o, t)
+
+with wf_observation : obs -> Prop :=
+| wf_obs :
+  forall
+    (o : obs),
+    wf_observation o
+.
+
+Inductive machine_strict_step : machine -> machine -> Prop :=
+| term_step :
+  forall m n
+    (o1 o2 : obs)
+    (t1 t2 : term),
+    step m n t1 t2 ->
+    machine_strict_step (o1 t1) (o2 t2)
+.
